We impose:
\begin{enumerate}
	\item \If $\locTransactionStarts_{i} = 1$ \Then:
        \begin{enumerate}
            \item $\indext_{i} = 0$ 
            \item $\indexx_{i} = 0$
        \end{enumerate}
    \item \If $\locTransactionStarts_{i} = 0$ \Then: 
        \begin{enumerate}
            \item $\indext_{i} = \indext_{i-1} + \lc_{i-1} \cdot \lt_{i-1}$ 
            \item $\indexx_{i} = \indexx_{i-1} + \lc_{i-1} \cdot \lx_{i-1}$. In other words, $\indext$ (resp. $\indexx$) resets to 0 at the begining of a new transaction, and increases by one after $\lc$ and $\lt$ (resp. $\lx$) is one.
        \end{enumerate}
      \item \If $\phaseRlpPrefix_{i} = 0$ \Then
        \begin{enumerate}
            \item $\rlptsize_{i} = \rlptsize_{i-1} - \lc_{i} \cdot \lt_{i} \cdot\limbsize_{i}$
            \item $\rlpxsize_{i} = \rlpxsize_{i-1} - \lc_{i} \cdot \lx_{i} \cdot\limbsize_{i}$
        \end{enumerate}
        \item $\toHashByProver_{i} = \lc_{i} \cdot \lx_{i}$
\end{enumerate}