The following constraints establish the staggered growth behaviour of
$\tliCounter$ and $\nonStackRowsCounter$
in conjunction with
$\tli$ and $\nonStackRows$.
We start with the latter:
\begin{enumerate}
	\item we require that $\tli$ and $\nonStackRows$ be \hubStamp-constant
	\item \If $\txExec _{i} = 0$ \Then
		\[
			\left\{ \begin{array}{lcl}
				\tli                 _{i} & = & 0 \\
				\nonStackRows        _{i} & = & 0 \\
			\end{array} \right.
		\]
\end{enumerate}
Setting
$\tli$ and $\nonStackRows$
in the ``nontrivial case'' (i.e. when $\txExec _{i} = 1$)
requires care, especially for $\nonStackRows$,
and will happen on an ``\evm{}-instruction per \evm{}-instruction'' basis
in section~(\ref{hub: instruction handling}).

We now venture forth with constraining
$\tliCounter$ and $\nonStackRowsCounter$:
\begin{enumerate}[resume]
	\item \If $\hubStamp_{i} \neq \hubStamp_{i - 1}$ \Then 
		\[
			\left\{ \begin{array}{lcl}
				\tliCounter          _{i} & = & 0 \\
				\nonStackRowsCounter _{i} & = & 0 \\
			\end{array} \right.
		\]
	\item \If $\txExec _{i} = 0$ \Then
		\[
			\left\{ \begin{array}{lcl}
				\tliCounter          _{i} & = & 0 \\
				\nonStackRowsCounter _{i} & = & 0 \\
			\end{array} \right.
		\]
	\item \If $\txExec _{i} = 1$ \Then
		\begin{enumerate}
			\item \If $\tliCounter_{i} \neq \tli_{i}$ \Then 
				\[
					\left\{ \begin{array}{lclr}
						\tliCounter          _{i + 1} & = & 1 + \tliCounter_{i}       \\
						\nonStackRowsCounter _{i + 1} & = & \nonStackRowsCounter _{i} \\
						\nonStackRowsCounter _{i    } & = & 0                          & (\sanityCheck) \\
					\end{array} \right.
				\]
			\item \If $\tliCounter_{i} = \tli_{i}$ \Then 
				\begin{enumerate}
					\item \If $\nonStackRowsCounter_{i} \neq \nonStackRows_{i}$ \Then
						\[
							\left\{ \begin{array}{lcl}
								\tliCounter          _{i + 1} & = & \tliCounter              _{i} \\
								\nonStackRowsCounter _{i + 1} & = & 1 + \nonStackRowsCounter _{i} \\
							\end{array} \right.
						\]
					\item \If $\nonStackRowsCounter_{i} = \nonStackRows_{i}$ \Then $\hubStamp_{i + 1} = 1 + \hubStamp_{i}$ (\sanityCheck)
				\end{enumerate}
		\end{enumerate}
\end{enumerate}
We further impose that
\begin{enumerate}[resume]
	\item \If $\txExec _{i} = 1$ \Then
		\begin{enumerate}
			\item \If $\nonStackRowsCounter _{i} =    0$ \Then $\peekStack _{i} = 1$
			\item \If $\nonStackRowsCounter _{i} \neq 0$ \Then $\peekStack _{i} = 0$
		\end{enumerate}
\end{enumerate}
