\begin{center}
	\boxed{\text{All constraints in this subsection assume that $\txAuth _{i} = 1$.}}
\end{center}
We impose the following:
\begin{enumerate}
	\item $\peekAuthorization _{i} + \peekAccount _{i} = 1$
	\item \If $\txAuth _{i - 1} = 0$ \Then $\peekAuthorization _{i} = 1$;
	\item \If $\peekAuthorization _{i} = 1$ \Then
		\begin{enumerate}
			\item \If $\authEcrecoverSuccess _{i} = 1$ \Then
				\begin{enumerate}
					\item $\txAuth      _{i + 1} = 1$
					\item $\peekAccount _{i + 1} = 1$
				\end{enumerate}
			\item \If $\authEcrecoverSuccess _{i} = 0$ \Then
				\begin{enumerate}
					\item $\txAuth      _{i + 1} = \peekAuthorization _{i + 1}$
				\end{enumerate}
		\end{enumerate}
	\item \If $\peekAccount _{i} = 1$ \Then
		\begin{enumerate}
			\item $\txAuth               _{i + 1} = \peekAuthorization _{i + 1}$
			\item we impose
				\[
					\standardDomSubStamps {
						anchorRow        = i      ,
						relOffset        = \rZero ,
						domOffset        = 0      ,
					}
				\]
		\end{enumerate}
\end{enumerate}
The above enforces that the \txAuth{}-phase is obtained by concatenating an arbitratry number the following building blocks
\begin{itemize}
	\item one $\peekAuthorization{}$-row
	\item one $\peekAuthorization{}$-row followed by one $\peekAccount$-row
\end{itemize}
